examples/leakage/rsort/rsort.sc
@@ -1,4 +1,4 @@
-//#OPTIONS_SECREC --implicitcoercions=defaultsc --backtrack=tryb --matching=gorderedm --promote=nop --verify=bothv --entrypoints="bitwise_rsort" --nodafnymodules
+//#OPTIONS_SECREC --implicitcoercions=defaultsc --backtrack=tryb --matching=gorderedm --promote=nop --verify=funcv --entrypoints="bitwise_rsort" --nodafnymodules
 
 module rsort;
 
@@ -17,18 +17,19 @@ domain private privatek;
 //@    (forall uint i ; (0 <= i && i < size(perm)) ==> 0 <= perm[i] && perm[i] < n)
 //@ }
 
-//@ function bool Distinct (uint[[1]] perm)
+//@ function bool DistinctUpTo (uint[[1]] perm, uint n)
 //@ context<>
 //@ noinline;
+//@ requires n <= size(perm);
 //@ {
-//@   (forall uint i,uint j; (i < size(perm)) && (j < size(perm)) && (i != j) ==> perm[i] != perm[j])
+//@   (forall uint i,uint j; (0 <= i && i < n) && (0 <= j && j < n) && (i != j) ==> perm[i] != perm[j])
 //@ }
 
 //@ function bool IsPerm (uint[[1]] perm)
 //@ context<>
 //@ inline;
 //@ {
-//@    IsPermUpTo(perm,size(perm)) && Distinct(perm)
+//@    IsPermUpTo(perm,size(perm)) && DistinctUpTo(perm,size(perm))
 //@ }
 
 //* Code
@@ -42,7 +43,7 @@ private bool[[2]] permute (private bool[[2]] xs, uint[[1]] perm)
     uint n1 = shape(xs)[0];
     uint n2 = shape(xs)[1];
     
-    private bool[[2]] ys (n1,n2);
+    havoc private bool[[2]] ys (n1,n2);
     for (uint i = 0; i < n1; i=i+1)
     //@ invariant 0 <= i && i <= n1;
     //@ invariant shape(ys) === shape(xs);
@@ -78,6 +79,19 @@ pair shuffle_pair (private bool [[2]] xs, private uint [[1]] ys)
     return ret;
 }
 
+private bool[[2]] apply_perm (private bool[[2]] bits, private uint[[1]] ord)
+//@ requires IsPerm(ord);
+//@ requires shape(bits)[0] === size(ord);
+//@ ensures shape(bits) === shape(\result);
+{
+    pair p = shuffle_pair(bits,ord);
+    bits = p.bits;
+    public uint[[1]] pord = declassify(p.ord);
+    bits = permute(bits,pord);
+    return bits;
+}
+
+
 private bool[[2]] bitwise_rsort (private bool[[2]] bits)
 {
     uint n = shape(bits)[0];
@@ -92,16 +106,28 @@ private bool[[2]] bitwise_rsort (private bool[[2]] bits)
         private uint[[1]] bitColMod2n (n);
         private uint n1;
         for (uint i = 0; i < n; i=i+1)
+        //@ invariant shape(bits) === {n,k};
         //@ invariant n == size(bitCol);
         //@ invariant n == size(bitColMod2n);
         //@ invariant 0 <= i && i <= n;
         //@ invariant n1 <= i;
         //@ invariant forall uint j; 0 <= j && j < i ==> bitColMod2n[j] <= 1;
+        //@ invariant sum(bitColMod2n[:i]) === n1;
         {
             bitColMod2n[i] = (uint) bitCol[i];
-            n1 = bitColMod2n[i] + n1;
+            private uint ubit = bitColMod2n[i];
+            //@ assert ubit <= 1;
+            //@ assert sum(bitColMod2n[:i]) === n1;
+            //@ SumSliceEnd(bitColMod2n,i);
+            n1 = ubit + n1;
+            //@ assert sum(bitColMod2n[:i+1]) === n1;
         }
         private uint n0 = classify(n) - n1;
+        //@ SliceEndEqual(bitColMod2n);
+        //@ SliceBeginEqual(bitColMod2n);
+        //@ assert sum(bitColMod2n) === n1;
+        //@ assert n1 <= n;
+        //@ assert n0 === n - sum(bitColMod2n);
         // counter for number of 0s
         private uint c0;
         // counter for number of 1s
@@ -113,21 +139,33 @@ private bool[[2]] bitwise_rsort (private bool[[2]] bits)
         //@ invariant shape(bits) === {n,k};
         //@ invariant n0 <= n;
         //@ invariant forall uint j; 0 <= j && j < n ==> bitColMod2n[j] <= 1;
-        //@ invariant n == size(bitColMod2n);
-        //@ invariant n == size(ord);
+        //@ invariant n === size(bitColMod2n);
+        //@ invariant n === size(ord);
         //@ invariant 0 <= i && i <= n;
         //@ invariant c0 + c1 == i;
-        //@ free invariant forall uint j ; (0 <= j && j < i) ==> 0 <= ord[j] && ord[j] < n;
-        //@ free invariant Distinct(ord);
+        //@ free invariant forall uint i ; 0 <= i && i < n ==> sum(bitColMod2n[:i]) <= size(bitColMod2n[:i]);
+        //@ free invariant forall uint i ; 0 <= i && i < n ==> sum(bitColMod2n[i:]) <= size(bitColMod2n[i:]);
+        //@ invariant c0 === i - sum(bitColMod2n[:i]);
+        //@ invariant c1 === sum(bitColMod2n[:i]);
+        //@ invariant n0 === c0 + n - i - sum(bitColMod2n[i:]);
+        //@ invariant forall uint j ; (0 <= j && j < i) ==> ord[j] < n;
+        //@ invariant forall uint j ; (0 <= j && j < i) ==> ((0 <= ord[j] && ord[j] < c0) || (n0 <= ord[j] && ord[j] < n0 + c1));
+        //@ invariant DistinctUpTo(ord,i);
         {
-            c0 = c0 + classify(1) - bitColMod2n[i];
-            c1 = c1 + bitColMod2n[i];
-            ord[i] = (classify(1)-bitColMod2n[i]) * c0 + bitColMod2n[i] * (n0 + c1);
+            //@ SumSliceBegin(bitColMod2n,i);
+            private uint ubit = bitColMod2n[i];
+            //@ assert ubit <= 1;
+            private uint nubit = classify(1)-ubit;
+            //@ assert nubit <= 1;
+            //@ assert 0 <= c0 && c0 < n;
+            //@ assert bitColMod2n[i] === 1 ==> (0 <= n0 + c1 && n0 + c1 < n);
+            ord[i] = nubit * c0 + ubit * (n0 + c1);
+            c0 = c0 + nubit;
+            c1 = c1 + ubit;
+            //@ SumSliceEnd(bitColMod2n,i);
+            //@ assert forall uint j ; (0 <= j && j < i) ==> ord[i] != ord[j];
         }
-        pair p = shuffle_pair(bits,ord);
-        bits = p.bits;
-        public uint[[1]] pord = declassify(p.ord);
-        bits = permute(bits,pord);
+        bits = apply_perm(bits,ord);
     }
     return bits;
 }
