src/Language/SecreC/TypeChecker/Type.hs-boot
@@ -22,11 +22,6 @@ isPublic :: ProverK loc m => loc -> Bool -> Type -> TcM m ()
 
 castTypeToType :: CastType GIdentifier Type -> Type
 
-toSetType :: ProverK loc m => loc -> Bool -> Type -> TcM m BaseType
-toMultisetType :: ProverK loc m => loc -> Type -> TcM m BaseType
-isPrivate :: ProverK loc m => loc -> Bool -> Type -> TcM m ()
-isPublic :: ProverK loc m => loc -> Bool -> Type -> TcM m ()
-
 typeToSecType :: (ProverK loc m) => loc -> Type -> TcM m SecType
 typeToBaseType :: (ProverK loc m) => loc -> Type -> TcM m BaseType
 typeToComplexType :: (ProverK loc m) => loc -> Type -> TcM m ComplexType
